Lott/Data/Substring.lean
@@ -1,8 +1,0 @@
-partial
-def Substring.dropPrefixes (s pre : Substring) : Substring :=
-  if pre.bsize = 0 then
-    s
-  else
-    match s.dropPrefix? pre with
-    | some s' => s'.dropPrefixes pre
-    | none => s
