Lott/Environment/MetaVar.lean
@@ -10,7 +10,8 @@ initialize metaVarExt : PersistentEnvExtension (Name × Bool) (Name × Bool) (Na
   addImportedFn := fun metaVarss =>
     return metaVarss.flatten.foldl (init := mkNameMap _) (fun acc (n, ln) => acc.insert n ln)
   addEntryFn := fun st (n, ln) => st.insert n ln
-  exportEntriesFn := RBMap.fold (cmp := Name.quickCmp) (init := #[]) fun acc n ln => acc.push (n, ln)
+  exportEntriesFn := Std.TreeMap.foldl (cmp := Name.quickCmp) (init := #[])
+    fun acc n ln => acc.push (n, ln)
 }
 
 end Lott
